Technical Reports/Automatic verification for the Bosque Programming Language/auto/firstdraft.el
@@ -1,0 +1,14 @@
+(TeX-add-style-hook
+ "firstdraft"
+ (lambda ()
+   (TeX-add-to-alist 'LaTeX-provided-class-options
+                     '(("llncs" "runningheads")))
+   (TeX-run-style-hooks
+    "latex2e"
+    "llncs"
+    "llncs10"
+    "graphicx")
+   (LaTeX-add-bibliographies
+    "bibliography/references"))
+ :latex)
+
