Technical Reports/Automatic verification for the Bosque Programming Language/bibliography/auto/references.el
@@ -1,0 +1,8 @@
+(TeX-add-style-hook
+ "references"
+ (lambda ()
+   (LaTeX-add-bibitems
+    "10.1007/978-3-319-41528-4_20"
+    "10.1007/978-3-540-78800-3_24"))
+ :bibtex)
+
